src/Translation.v
@@ -1,0 +1,172 @@
+Require Import String.
+Require Import List.
+Require Import Bool.
+Require Import BinNums.
+From Coq Require Import Logic.FunctionalExtensionality.
+Import ListNotations.
+From hahn Require Import HahnBase.
+From Coq Require Import Classes.EquivDec.
+From Coq Require Import Classes.RelationClasses.
+
+Require Import Cypher.
+Require Import Semantics.
+Require Import PropertyGraph.
+Require Import ExecutionPlan.
+Require Import Maps.
+Require Import Utils.
+
+Import PropertyGraph.
+Import ExecutionPlan.
+Import FilterMode.
+Import ExpandMode.
+
+Section translate_pattern.
+  Import Pattern.
+
+  Definition translate_pvertex pv plan : ExecutionPlan.t :=
+    match vlabel pv with
+    | Some l => FilterByLabel Vertices (vname pv) l plan
+    | None => plan
+    end.
+
+  Definition translate_pedge pe plan : ExecutionPlan.t :=
+    match elabel pe with
+    | Some l => FilterByLabel Edges (ename pe) l plan
+    | None => plan
+    end.
+
+  Fixpoint translate_pattern (pi : Pattern.t) : ExecutionPlan.t :=
+    match pi with
+    | Pattern.start pv => 
+        translate_pvertex pv (ScanVertices (vname pv))
+    | Pattern.hop pi pe pv =>
+      let plan := translate_pattern pi in
+      let plan :=
+        if (In_decb (vname pv) (dom_vertices pi)) then
+          Expand Into (vname (last pi)) (ename pe) (vname pv) (edir pe) plan
+        else
+          Expand All (vname (last pi)) (ename pe) (vname pv) (edir pe) plan
+      in translate_pvertex pv (translate_pedge pe plan)
+    end.
+End translate_pattern.
+
+Ltac normilize_bool :=
+  repeat match goal with
+  | [ H : negb _ = true |- _ ] => rewrite negb_true_iff in H
+  | [ H : negb _ <> true |- _ ] => rewrite negb_true_iff in H
+  | [ H : _ = false |- _ ] => rewrite <- not_true_iff_false in H
+  | [ H : _ <> false |- _ ] => rewrite -> not_false_iff_true in H
+  | [ H : (In_decb _ _) = true |- _ ] => rewrite -> In_decb_true_iff in H
+  | [ H : (In_decb _ _) <> true |- _ ] => rewrite -> In_decb_true_iff in H
+  end.
+
+Theorem translate_pattern__type_of pi n (Hwf : Pattern.wf pi) :
+  (In n (Pattern.dom_edges pi) <-> type_of (translate_pattern pi) n = Some Value.GEdgeT) /\
+  (In n (Pattern.dom_vertices pi) <-> type_of (translate_pattern pi) n = Some Value.GVertexT).
+Proof.
+  all: induction pi; simpls.
+  all: unfold Pattern.wf in *.
+  all: unfold translate_pvertex.
+  all: unfold translate_pedge.
+
+  { split; split; ins; desf; simpls.
+    all: autounfold with unfold_pat in *.
+    all: desf; simpls.
+    all: eauto with pattern_wf_db.
+    all: unfold complement, equiv in *; contradiction. }
+
+  split.
+  all: desf; simpls.
+  all: normilize_bool.
+  all: split; ins; desf.
+
+  all: try now apply update_eq.
+  all: try rewrite update_neq.
+  all: try now apply update_eq.
+  all: try rewrite update_neq.
+  all: try (apply IHpi; [ split | ]; now eauto with pattern_wf_db).
+
+  all: try now (intros ?; exfalso; subst; eauto with pattern_wf_db).
+  all: try now (intros ?; exfalso; subst; simple eapply NoDup_cons_l; eassumption).
+
+  all: autounfold with unfold_pat in *.
+  all: desf; simpls.
+  all: try (left; now eauto with pattern_wf_db).
+  all: right; apply IHpi; [ split | ]; now eauto with pattern_wf_db.
+Qed.
+
+Corollary translate_pattern__type_of_GVertexT pi n (Hwf : Pattern.wf pi) :
+  (In n (Pattern.dom_vertices pi) <-> type_of (translate_pattern pi) n = Some Value.GVertexT).
+Proof. edestruct translate_pattern__type_of; eassumption. Qed.
+
+Corollary translate_pattern__type_of_GEdgeT pi n (Hwf : Pattern.wf pi) :
+  (In n (Pattern.dom_edges pi) <-> type_of (translate_pattern pi) n = Some Value.GEdgeT).
+Proof. edestruct translate_pattern__type_of; eassumption. Qed.
+
+Corollary translate_pattern__type_of_None pi n (Hwf : Pattern.wf pi)
+  (HIn_vertices : ~ In n (Pattern.dom_vertices pi))
+  (HIn_edges    : ~ In n (Pattern.dom_edges pi)) :
+    type_of (translate_pattern pi) n = None.
+Proof.
+  edestruct type_of_types as [H | [H | H]].
+  - eapply translate_pattern__type_of_GVertexT in H; try eassumption.
+    apply HIn_vertices in H. contradiction.
+  - eapply translate_pattern__type_of_GEdgeT in H; try eassumption.
+    apply HIn_edges in H. contradiction.
+  - assumption.
+Qed.
+
+Corollary translate_pattern__type_of_None_iff pi n (Hwf : Pattern.wf pi) :
+  ~ In n (Pattern.dom_vertices pi) /\ ~ In n (Pattern.dom_edges pi) <->
+    type_of (translate_pattern pi) n = None.
+Proof.
+  split.
+  { intros [? ?]. apply translate_pattern__type_of_None; assumption. }
+  ins. split.
+  all: intros contra.
+  1: apply translate_pattern__type_of_GVertexT in contra; try assumption.
+  2: apply translate_pattern__type_of_GEdgeT in contra; try assumption.
+  all: congruence.
+Qed.
+
+Theorem translate_pattern_wf pi (Hwf : Pattern.wf pi) :
+  ExecutionPlan.wf (translate_pattern pi).
+Proof.
+  induction pi; simpls.
+  2: assert (Pattern.wf pi) by (eapply Pattern.hop_wf; eassumption).
+  all: unfold translate_pvertex, translate_pedge.
+  all: desf; simpls.
+  all: normilize_bool.
+  all: repeat split.
+  all: try apply translate_pattern__type_of_GVertexT; try assumption.
+  all: try apply translate_pattern__type_of_None; try assumption.
+  all: eauto with pattern_wf_db.
+
+  all: autounfold with unfold_pat in *.
+  all: desf.
+  all: unfold complement, equiv in *.
+  all: eauto with pattern_wf_db.
+  all: try contradiction.
+  all: try apply translate_pattern__type_of_GVertexT; try assumption.
+  all: try (exfalso; simple eapply Pattern.wf__pe_neq_pv; eassumption).
+  all: try (exfalso; simple eapply Pattern.wf__pv_neq_pe; eassumption).
+Qed.
+
+Module EvalQueryImpl (S : ExecutionPlan.Spec).
+  Module EvalPlanImpl := EvalPlan S.
+  Import S.
+  Import EvalPlanImpl.
+
+  Definition eval_pattern (graph : PropertyGraph.t) (pi : Pattern.t) : option BindingTable.t :=
+    let plan := translate_pattern pi in
+      EvalPlanImpl.eval graph plan.
+  
+  Theorem eval_pattern__wf graph pi
+    (Hwf_g : PropertyGraph.wf graph) (Hwf : Pattern.wf pi) :
+      exists table', eval_pattern graph pi = Some table'.
+  Proof.
+    eapply eval_wf.
+    1: apply translate_pattern_wf.
+    all: assumption.
+  Qed.
+End EvalQueryImpl.
